# Tester and Modell, 1997

$d\underline{U}=Td\underline{S}-Pd\underline{V}+\sum_1^n \mu_i dN_i$

$U=f(\underline{S},\underline{V},N_1...N_n)$

$T = \left( \frac{\partial \underline{U}}{\partial S}\right)_{\underline{V},N}$

$\mu_i = \left( \frac{\partial \underline{U}}{\partial N_i}\right)_{\underline{S},\underline{V},N_{j[i]}}$

$[\underline{\underline{a}}]=[\underline{z}][\underline{b}]$

# O'Connell and Haile, 

$\bar{G}_i^\mathrm{E} \left( T, P, \left\{ x \right\} \right)$

$\bar{G}_i^\mathrm{E} \left( T, P, \left\{ x \right\} \right)$

$P\left(T,V,x_1,x_2,...\right)$

$\left( \frac{\partial {U}}{\partial S}\right)_{Vx}$

$\frac{\partial}{\partial N_i}\left[ \left( \frac{\partial G}{\partial P}\right)_{TN} \right]_{TPN_{j \neq i}}=\bar{V}_i$
